secure_api/box/Box.PlainAE.fst
@@ -15,7 +15,7 @@ type bytes = seq UInt8.t
    The protected plaintext type of AE. It is associated with an id and acts as a wrapper around a protected pkae plaintext.
    The ids associated with both plaintexts must be equal.
 *)
-abstract type protected_ae_plain (i:id{AE_id? i}) = p:protected_pkae_plain{get_index p = i}
+abstract type protected_ae_plain (i:id{AE_id? i}) = p:protected_pkae_plain i
 
 (**
    The unprotected plaintext type.
@@ -26,7 +26,7 @@ type ae_plain = b:bytes{Seq.length b / Spec.Salsa20.blocklen < pow2 32}
    This function can bypass the abstraction protection of the protected plaintext type. However, this is only possible
    if ae_ind_cpa is not idealized, or if the id associated with the plaintext is dishonest.
 *)
-val repr: #i:id{AE_id? i} -> p:protected_ae_plain i{not ae_ind_cpa \/ (dishonest i)} -> Tot (ae_plain)
+val repr: #i:id{AE_id? i} -> p:protected_ae_plain i{not ae_ind_cpa \/ dishonest i} -> Tot (ae_plain)
 let repr #i p =
     PlainBox.repr p
 
@@ -34,7 +34,7 @@ let repr #i p =
    This function allows the creation of protected plaintexts. Protected plaintexts can only be created by the adversary if
    either ae_int_cca is not idealized or of the id associated with the newly created plaintext is dishonest.
 *)
-val coerce: #i:id{AE_id? i} -> p:ae_plain{not ae_ind_cca \/ (dishonest i)} -> Tot (protected_ae_plain i)
+val coerce: #i:id{AE_id? i} -> p:ae_plain{not ae_int_ctxt \/ (dishonest i)} -> Tot (protected_ae_plain i)
 let coerce #i p =
   PlainBox.coerce #i p
 
@@ -42,18 +42,18 @@ let coerce #i p =
    This is a helper function used by the top-level box function to encapsulate the payload before
    passing it on to AE.encrypt.
 *)
-val ae_message_wrap: #i:id{AE_id? i} -> p:protected_pkae_plain{get_index p = i} -> Tot (protected_ae_plain i)
+val ae_message_wrap: #i:id{AE_id? i} -> p:protected_pkae_plain i -> Tot (protected_ae_plain i)
 let ae_message_wrap #i p = p
 
 (**
    This is the reverse function to ae_message_wrap. box_open uses it to extract a
    protected ae payload.
 *)
-val ae_message_unwrap: #i:id{AE_id? i} -> p:protected_ae_plain i -> Tot (p:protected_pkae_plain{get_index p = i})
+val ae_message_unwrap: #i:id{AE_id? i} -> p:protected_ae_plain i -> Tot (p:protected_pkae_plain i)
 let ae_message_unwrap #i p = p
 
   (**
      A helper function to obtain the length of a protected plaintext.
      *)
 val length: #i:id{AE_id? i} -> (protected_ae_plain i) -> Tot (n:nat {n / Spec.Salsa20.blocklen < pow2 32})
-let length #i p = PlainBox.length p
+let length #i p = PlainBox.length #i p
